Generalized theorems for typed optimization

erasure/theories/Typed/ExtractionCorrectness.v
@@ -458,6 +458,111 @@ Proof.
       now eapply PCUICWfEnvImpl.wf_fresh_globals.
 Qed.
 
+From Coq Require Import String.
+Local Open Scope string_scope.
+
+Import MCMonadNotation.
+
+Definition compute_masks overridden_masks do_trim_const_masks do_trim_ctor_masks Σ : result dearg_set bytestring.string :=
+  let (const_masks, ind_masks) := Utils.timed "Dearg analysis" (fun _ => analyze_env overridden_masks Σ) in
+  let const_masks := (if do_trim_const_masks then trim_const_masks else id) const_masks in
+  let ind_masks := (if do_trim_ctor_masks then trim_ind_masks else id) ind_masks in
+  throwIf (negb (is_expanded_env ind_masks const_masks Σ))
+    "Erased environment is not expanded enough for dearging to be provably correct"%bs ;;
+  throwIf (negb (valid_masks_env ind_masks const_masks Σ))
+    "Analysis produced masks that ask to remove live arguments"%bs ;;
+  Ok (Build_dearg_set const_masks ind_masks).
+
+Definition dearg_env masks Σ :=
+  debox_env_types (dearg_env masks.(ind_masks) masks.(const_masks) Σ).
+
+Import PCUICWfEnvImpl.
+
+Program Definition dearg_term {Σ} (wfΣ : ∥wf_ext Σ∥) (masks : dearg_set) (t : PCUICAst.term) (w : welltyped Σ [] t) : term :=
+  let wfext := @abstract_make_wf_env_ext _ (optimized_abstract_env_impl (guard := Erasure.fake_guard_impl_instance)) (PCUICWfEnvImpl.build_wf_env_from_env Σ (map_squash fst wfΣ)) Σ.2 _ in
+  dearg masks.(ind_masks) masks.(const_masks) (erase _ wfext (normalization_in := _) [] t _).
+  Next Obligation.
+    refine (let 'sq wfΣ := wfΣ in let nin := Erasure.fake_normalization Σ wfΣ in _).
+    eapply nin. destruct Σ. apply H.
+  Qed.
+
+  Next Obligation.
+    destruct Σ. apply w.
+  Qed.
+
+Theorem extract_correct_gen
+        (H := EWellformed.all_env_flags)
+        (wfl := opt_wcbv_flags)
+        (Σ : P.global_env_ext) (wfΣ : ∥wf_ext Σ∥)
+        t v ignored exΣ masks :
+  axiom_free Σ ->
+  forall wt : welltyped Σ [] t,
+  forall wv : welltyped Σ [] v,
+  Σ p⊢ t ⇓ v ->
+  (isErasable Σ [] t -> False) ->
+  (forall k, ignored k = false) ->
+  let t' := dearg_term wfΣ masks t wt in
+  extract_pcuic_env
+    (pcuic_args extract_within_coq)
+    Σ (wf_squash wfΣ) (EAstUtils.term_global_deps t') ignored = Ok exΣ ->
+  compute_masks (fun _ => None) true true exΣ = Ok masks ->
+  ∥trans_env exΣ e⊢ t' ⇓ dearg_term wfΣ masks v wv ∥.
+Proof.
+  intros ax [T wt] wv ev not_erasable no_ignores ex.
+  cbn -[dearg_transform] in *.
+  destruct dearg_transform eqn:dt; cbn -[dearg_transform] in *; [|congruence].
+  intros [=->].
+  destruct wfΣ.
+  unfold dearg_term.
+  set (e := abstract_make_wf_env_ext _ _ _).
+  pose proof (abstract_env_ext_exists e) as [[Σe he]].
+  unfold dearg_term in ex.
+  match goal with
+  [H := context [ @erase ?X_type ?X ?nin ?Γ t ?wt ] |- _ ] =>
+   pose proof (@erases_erase X_type X nin Γ t wt _ he)
+  end.
+  cbn in he. subst Σe. destruct Σ as [Σ univs]; cbn [fst snd] in *.
+  eapply erases_correct with
+    (Σ' := trans_env (Erasure.erase_global_decls_deps_recursive (PCUICAst.PCUICEnvironment.declarations Σ)
+               (PCUICAst.PCUICEnvironment.universes Σ) _ _
+               _ ignored)) in ev as (erv&erase_to&[erev]);eauto.
+  2:{ now eexists. }
+  intros Σex.
+  * move: dt. unfold dearg_transform. eapply dearg_correct.
+  2:{ unshelve eapply (erases_erase (X_type := (optimized_abstract_env_impl (guard := Erasure.fake_guard_impl_instance)))). exact e. 3:now destruct Σ.
+    * intros. pose proof (abstract_env_ext_irr _ he H0). subst Σ0. now apply Erasure.fake_normalization.
+    * intros Σ0 he'; pose proof (abstract_env_ext_irr _ he he'); subst Σ0. cbn in he, he'. subst Σe. now destruct Σ. }
+  3:{ intros hm.
+
+  eapply dearg_correct.
+  + depelim erase_to;[|easy].
+    constructor.
+    eapply dearg_transform_correct; eauto.
+    clear dt.
+    eapply (@optimize_correct _ _ _ (tConst kn) (tConstruct ind c []));eauto.
+    * remember (Erasure.erase_global_decls_deps_recursive _ _ _ _ _ _) as eΣ.
+      assert (EWellformed.wf_glob (trans_env eΣ)).
+      { subst eΣ. now eapply wf_erase_global_decls_recursive. }
+      now apply EWellformed.wellformed_closed_env.
+    * eapply wf_erase_global_decls_recursive; auto.
+  + now eexists.
+  + eapply inversion_Const in wt as (?&?&?&?&?); auto.
+    clear dt.
+    eapply global_erased_with_deps_erases_deps_tConst; eauto.
+    destruct Σ as [Σ0 univ_decls].
+    destruct Σ0 as [univs Σ1].
+    apply wf_ext_wf in w as w1. cbn.
+    eapply erase_global_decls_deps_recursive_correct;eauto.
+    * unfold PCUICAst.declared_constant in *.
+      cbn.
+      intros ? ->%KernameSet.singleton_spec;cbn in *.
+      intros eq. set (env := {| PEnv.declarations := Σ1 |}) in *.
+      eapply (lookup_global_In_wf _ env) in d; eauto.
+    * now apply KernameSet.singleton_spec.
+    Unshelve. eapply fresh_globals_erase_global_decl_rec.
+      now eapply PCUICWfEnvImpl.wf_fresh_globals.
+Qed.
+
 (* Print Assumptions extract_correct. *)
 
 (** There are some assumptions of which almost all are in MetaCoq.
