erasure-plugin/theories/ETransform.v
@@ -204,7 +204,9 @@ Program Definition erase_transform {guard : abstract_guard_impl} : Transform.t _
      /\ NormalizationIn_erase_pcuic_program_1 p.1
      /\ NormalizationIn_erase_pcuic_program_2 p.1 ;
    transform p hp := let nhs := proj2 (proj2 hp) in
-                     @erase_program guard p (proj1 nhs) (proj2 nhs) (proj1 hp) ;
+                     @erase_
+
+                     program guard p (proj1 nhs) (proj2 nhs) (proj1 hp) ;
     post p := [/\ wf_eprogram_env all_env_flags p & EEtaExpandedFix.expanded_eprogram_env p];
    obseq p hp p' v v' := let Σ := p.1 in Σ ;;; [] |- v ⇝ℇ v' |}.
 
@@ -380,14 +382,14 @@ Qed.
 Instance rebuild_wf_env_extends {fl : EWcbvEval.WcbvFlags} {efl : EEnvFlags} with_exp :
   TransformExt.t (rebuild_wf_env_transform with_exp) (fun p p' => extends p.1 p'.1) (fun p p' => extends p.1 p'.1).
 Proof.
-  red. intros p p' pr pr' ext. red. now rewrite /transform /=. 
+  red. intros p p' pr pr' ext. red. now rewrite /transform /=.
 Qed.
 
 #[global]
 Instance rebuild_wf_env_extends' {fl : EWcbvEval.WcbvFlags} {efl : EEnvFlags} with_exp :
   TransformExt.t (rebuild_wf_env_transform with_exp) extends_eprogram extends_eprogram_env.
 Proof.
-  red. intros p p' pr pr' [? ?]. now rewrite /transform /=. 
+  red. intros p p' pr pr' [? ?]. now rewrite /transform /=.
 Qed.
 
 Program Definition remove_params_optimization {fl : EWcbvEval.WcbvFlags} {wcon : EWcbvEval.with_constructor_as_block = false}
@@ -431,7 +433,7 @@ Instance remove_params_extends' {fl : EWcbvEval.WcbvFlags}  {wcon : EWcbvEval.wi
   TransformExt.t (remove_params_optimization (wcon:=wcon)) extends_eprogram_env extends_eprogram.
 Proof.
   red. intros p p' pr pr' [ext eq]. rewrite /transform /= /strip_program. rewrite eq.
-  red. cbn -[strip_env strip]. split. eapply strip_extends_env => //. apply pr. apply pr'.  
+  red. cbn -[strip_env strip]. split. eapply strip_extends_env => //. apply pr. apply pr'.
   cbn -[strip_env strip]. eapply strip_extends => //. apply pr'. rewrite -eq. apply pr.
 Qed.
 
@@ -470,7 +472,7 @@ Instance remove_params_fast_extends {fl : EWcbvEval.WcbvFlags}  {wcon : EWcbvEva
   (efl := all_env_flags):
   TransformExt.t (remove_params_fast_optimization (wcon:=wcon)) (fun p p' => extends p.1 p'.1) (fun p p' => extends p.1 p'.1).
 Proof.
-  red. intros p p' pr pr' ext. rewrite /transform /=. 
+  red. intros p p' pr pr' ext. rewrite /transform /=.
   rewrite -!ERemoveParams.Fast.strip_env_fast.
   eapply strip_extends_env => //. apply pr. apply pr'.
 Qed.
@@ -523,7 +525,7 @@ Qed.
 Instance remove_match_on_box_extends'  {fl : WcbvFlags} {wcon : with_constructor_as_block = false} {efl : EEnvFlags} {hastrel : has_tRel} {hastbox : has_tBox} :
   TransformExt.t (remove_match_on_box_trans (wcon:=wcon) (hastrel := hastrel) (hastbox := hastbox)) extends_eprogram_env extends_eprogram.
 Proof.
-  red. intros p p' pr pr' [ext eq]. rewrite /transform /= /remove_match_on_box_program. split. 
+  red. intros p p' pr pr' [ext eq]. rewrite /transform /= /remove_match_on_box_program. split.
   eapply remove_match_on_box_extends_env => //. apply pr. apply pr'.
   rewrite -eq.
   eapply wellformed_remove_match_on_box_extends; eauto. apply pr. apply pr'.
@@ -567,7 +569,7 @@ Instance inline_projections_optimization_extends' {fl : WcbvFlags} {wcon : EWcbv
   {hastrel : has_tRel} {hastbox : has_tBox} :
   TransformExt.t (inline_projections_optimization (wcon:=wcon) (hastrel := hastrel) (hastbox := hastbox)) extends_eprogram_env extends_eprogram.
 Proof.
-  red. intros p p' pr pr' [ext eq]. rewrite /transform /= /optimize_program /=. split. 
+  red. intros p p' pr pr' [ext eq]. rewrite /transform /= /optimize_program /=. split.
   eapply optimize_extends_env => //. apply pr. apply pr'.
   rewrite -eq.
   eapply wellformed_optimize_extends; eauto. apply pr. apply pr'.
@@ -616,7 +618,7 @@ Instance constructors_as_blocks_extends' (efl : EEnvFlags)
   TransformExt.t (constructors_as_blocks_transformation (has_app := has_app) (has_rel := has_rel) (hasbox := hasbox) (has_pars := has_pars) (has_cstrblocks := has_cstrblocks))
   extends_eprogram_env extends_eprogram.
 Proof.
-  red. intros p p' pr pr' [ext eq]. rewrite /transform /=. split. 
+  red. intros p p' pr pr' [ext eq]. rewrite /transform /=. split.
   eapply transform_blocks_env_extends => //. apply pr. apply pr'.
   unfold transform_blocks_program => /=.
   rewrite -eq.
